theories/base_logic/lib/cancelable_invariants.v
@@ -92,12 +92,13 @@ Section proofs.
   Qed.
 
   Global Instance into_inv_cinv N γ P : IntoInv (cinv N γ P) N.
-  Global Instance elim_inv_cinv p γ E N P P' Q Q' :
-    ElimModal True (|={E,E∖↑N}=> (▷ P ∗ cinv_own γ p) ∗ (▷ P ={E∖↑N,E}=∗ True))%I P' Q Q' →
-    ElimInv (↑N ⊆ E) (cinv N γ P) (cinv_own γ p) P' Q Q'.
+  Global Instance elim_inv_cinv p γ E N P Q Q' :
+    (∀ R, ElimModal True (|={E,E∖↑N}=> R) R Q Q') →
+    ElimInv (↑N ⊆ E) (cinv N γ P) (cinv_own γ p)
+      (▷ P ∗ cinv_own γ p) (▷ P ={E∖↑N,E}=∗ True) Q Q'.
   Proof.
     rewrite /ElimInv /ElimModal. iIntros (Helim ?) "(#H1&Hown&H2)".
-    iApply Helim; auto. iFrame "H2".
+    iApply (Helim with "[- $H2]"); first done.
     iMod (cinv_open E N γ p P with "[#] [Hown]") as "(HP&Hown&Hclose)"; auto. 
     by iFrame.
   Qed.
