theories/base_logic/lib/na_invariants.v
@@ -112,13 +112,13 @@ Section proofs.
   Qed.
 
   Global Instance into_inv_na p N P : IntoInv (na_inv p N P) N.
-  Global Instance elim_inv_na p F E N P P' Q Q':
-    ElimModal True (|={E}=> (▷ P ∗ na_own p (F∖↑N)) ∗ (▷ P ∗ na_own p (F∖↑N) ={E}=∗ na_own p F))%I
-              P' Q Q' →
-    ElimInv (↑N ⊆ E ∧ ↑N ⊆ F) (na_inv p N P) (na_own p F) P' Q Q'.
+  Global Instance elim_inv_na p F E N P Q Q':
+    (∀ R, ElimModal True (|={E}=> R)%I R Q Q') →
+    ElimInv (↑N ⊆ E ∧ ↑N ⊆ F) (na_inv p N P) (na_own p F)
+      (▷ P ∗ na_own p (F∖↑N)) (▷ P ∗ na_own p (F∖↑N) ={E}=∗ na_own p F) Q Q'.
   Proof.
     rewrite /ElimInv /ElimModal. iIntros (Helim (?&?)) "(#H1&Hown&H2)".
-    iApply Helim; auto. iFrame "H2".
+    iApply (Helim with "[- $H2]"); first done.
     iMod (na_inv_open p E F N P with "[#] [Hown]") as "(HP&Hown&Hclose)"; auto. 
     by iFrame.
   Qed.
