theories/proofmode/coq_tactics.v
@@ -1171,19 +1171,19 @@ Proof.
 Qed.
 
 (** * Invariants *)
-Lemma tac_inv_elim Δ Δ' i j φ p P Pin Pout Q Q' :
+Lemma tac_inv_elim Δ Δ' i j φ p P Pin Pout Pclose Q Q' :
   envs_lookup_delete false i Δ = Some (p, P, Δ') →
-  ElimInv φ P Pin Pout Q Q' →
+  ElimInv φ P Pin Pout Pclose Q Q' →
   φ →
   (∀ R, ∃ Δ'',
-    envs_app false (Esnoc Enil j (Pin -∗ (Pout -∗ Q') -∗ R)%I) Δ' = Some Δ'' ∧
+    envs_app false (Esnoc Enil j (Pin -∗ (Pout -∗ Pclose -∗ Q') -∗ R)%I) Δ' = Some Δ'' ∧
     envs_entails Δ'' R) →
   envs_entails Δ Q.
 Proof.
   rewrite envs_entails_eq=> /envs_lookup_delete_Some [? ->] ?? /(_ Q) [Δ'' [? <-]].
   rewrite (envs_lookup_sound' _ false) // envs_app_singleton_sound //; simpl.
-  apply wand_elim_r', wand_mono; last done.
-  apply wand_intro_r, wand_intro_r. rewrite affinely_persistently_if_elim -assoc. auto.
+  apply wand_elim_r', wand_mono; last done. apply wand_intro_r, wand_intro_r.
+  rewrite affinely_persistently_if_elim -assoc wand_curry. auto.
 Qed.
 End bi_tactics.
 
